operator overloading

bedrock2/src/bedrock2/OperatorOverloading.v
@@ -2,178 +2,69 @@ Require Import Coq.ZArith.ZArith.
 Require Import coqutil.Map.Interface.
 Require Import coqutil.Word.Interface.
 Require Import bedrock2.Map.SeparationLogic.
+Require Export coqutil.Datatypes.OperatorOverloading.
+Require Export bedrock2.ListIndexNotations.
+
+#[export] Instance MulSepClause{K V: Type}{M: map.map K V}(a b: @map.rep K V M -> Prop)
+  : Multiplication a b (sep a b) | 10 := {}.
+
+#[export] Instance MulSepClauseType{K V: Type}{M: map.map K V}(a b: @map.rep K V M -> Prop)
+  : @Multiplication (M -> Prop) (M -> Prop) (M -> Type) a b (sep a b) | 20 := {}.
+
+Local Set Warnings "-notation-overridden".
+Notation "a * b" := (sep a b) (only printing) : type_scope.
+Local Set Warnings "notation-overridden".
+
+Notation "a * b" := (sep a b) (only printing) : oo_scope.
+
+Notation "a * b" := (infer! Multiplication a b) (only parsing) : type_scope.
 
 
-Ltac get_type x :=
-  let tx := type of x in
-  let __ := match constr:(Set) with
-            | _ => tryif has_evar tx
-                   then fail 1 "type of" x "should be fully determined, but is" tx
-                   else idtac
-            end in
-  tx.
+Require Import bedrock2.Scalars.
 
-(* might insert a coercion, or use subsumption to turn `nat: Set` into `nat: Type` *)
-Ltac has_type x T :=
-  tryif (let _ := constr:(x: T) in idtac) then idtac
-  else fail 0 x "does not have type" T.
+Class PointsTo{width: Z}{word: word.word width}{mem: map.map word Byte.byte}{V: Type}
+      (addr: word)(val: V)(pred: mem -> Prop) := {}.
 
-Ltac binop cl x y :=
-  (* At the moment, we require both the type of x and y to be fully determined
-     (no evars), but later we might be more adventurous and allow the type of
-     one operand to determine the type of the other.
-     But then we'll have to reconsider what to do about coercions. *)
-  let tx := get_type x in
-  let ty := get_type y in
-  (* unify instead of constr_eq because has_type also uses unification *)
-  tryif unify tx ty then
-    (* beta gets rid of cast and of eta expansion in case of prod used for Set *)
-    let r := eval cbv beta in ((_: cl tx) x y) in exact r
-  else
-    tryif has_type x ty then
-      tryif has_type y tx then
-        fail "bidirectional coercion between" tx "and" ty
-             "makes" cl "of" x "and" y "ambiguous"
-      else
-        (* will coerce type of x to ty *)
-        let r := eval cbv beta in ((_: cl ty) x y) in exact r
-    else
-      tryif has_type y tx then
-        (* will coerce type of y to tx *)
-        let r := eval cbv beta in ((_: cl tx) x y) in exact r
-      else
-        fail "operands" x "and" y "have incompatible types" tx "and" ty.
+(* Precedence: `*` is at level 40, and we want to bind stronger than `*`, and moreover,
+   `^` is at level 30, and for consistency, we also want to bind stronger than `^`,
+   so we choose 25. *)
+Notation "a |-> v" := (infer! PointsTo a v)
+  (at level 25, only parsing).
+
+#[export] Instance PointsToScalar{width}{word: word.word width}{mem: map.map word Byte.byte}
+ (a v: word): PointsTo a v (scalar a v) := {}.
+
+Notation "a |-> v" := (scalar a v)
+  (at level 25, format "'[  ' a  |->  '/' v ']'", only printing).
+
+Require Import bedrock2.Array.
 
 
-Declare Scope oo_scope.
-Local Open Scope oo_scope.
+Section TestNotations.
+  Context {width: Z} {word: word.word width} {mem: map.map word Byte.byte}.
+  Local Open Scope oo_scope.
 
-Definition Multiplication(T: Type) := T -> T -> T.
-Existing Class Multiplication.
-#[export] Hint Mode Multiplication + : typeclass_instances.
+  Goal forall (P Q: mem -> Prop), P * Q = sep P Q. intros. srefl. Abort.
+  Goal forall (P Q: mem -> Prop), Lift1Prop.iff1 (P * Q) (sep P Q).
+    intros. reflexivity.
+  Abort.
 
-#[export] Hint Extern 1 (Multiplication nat) => exact Nat.mul : typeclass_instances.
-#[export] Hint Extern 1 (Multiplication N) => exact N.mul : typeclass_instances.
-#[export] Hint Extern 1 (Multiplication Z) => exact Z.mul : typeclass_instances.
-#[export] Hint Extern 1 (Multiplication Set) => exact prod : typeclass_instances.
-#[export] Hint Extern 1 (Multiplication Prop) => exact prod : typeclass_instances.
-#[export] Hint Extern 1 (Multiplication Type) => exact prod : typeclass_instances.
-#[export] Hint Extern 1 (Multiplication (@word.rep ?wi ?wo)) =>
-  exact (@word.mul wi wo) : typeclass_instances.
-#[export] Hint Extern 1 (Multiplication (@map.rep ?K ?V ?M -> Prop)) =>
-  exact (@sep K V M) : typeclass_instances.
+  Goal forall (P Q R: mem -> Prop), P * Q * R = sep (sep P Q) R. intros. srefl. Abort.
 
-Notation "x * y" := (ltac:(binop Multiplication x y)) (only parsing) : oo_scope.
-Notation "x * y" := (Nat.mul x y) (only printing): oo_scope.
-Notation "x * y" := (N.mul x y) (only printing): oo_scope.
-Notation "x * y" := (Z.mul x y) (only printing): oo_scope.
-Notation "x * y" := (prod x y) (only printing): oo_scope.
-Notation "x * y" := (word.mul x y) (only printing): oo_scope.
-Notation "x * y" := (sep x y) (only printing): oo_scope.
-
-
-Definition Addition(T: Type) := T -> T -> T.
-Existing Class Addition.
-#[export] Hint Mode Addition + : typeclass_instances.
-
-#[export] Hint Extern 1 (Addition nat) => exact Nat.add : typeclass_instances.
-#[export] Hint Extern 1 (Addition N) => exact N.add : typeclass_instances.
-#[export] Hint Extern 1 (Addition Z) => exact Z.add : typeclass_instances.
-#[export] Hint Extern 1 (Addition (@word.rep ?wi ?wo)) =>
-  exact (@word.add wi wo) : typeclass_instances.
-
-Notation "x + y" := (ltac:(binop Addition x y)) (only parsing) : oo_scope.
-Notation "x + y" := (Nat.add x y) (only printing): oo_scope.
-Notation "x + y" := (N.add x y) (only printing): oo_scope.
-Notation "x + y" := (Z.add x y) (only printing): oo_scope.
-Notation "x + y" := (word.add x y) (only printing): oo_scope.
-
-(* Check ((_: nat) * (_: nat))
-   fails, but here are workarounds: *)
-Notation "?? x : T 'in' b" := (match _: T with
-                               | x => b
-                               end)
-  (at level 10, right associativity, x at level 0, T at level 9, b at level 9, only parsing)
-    : oo_scope.
-
-Goal False.
-  epose ((_: nat) - (_: nat)). (* succeeds because we haven't overloaded - yet *)
-
-  assert_fails (epose ((_:nat) * (_:nat))). (* Cannot infer this placeholder of type "nat" *)
-
-  epose (let a: nat := _ in let b: nat := _ in a * b).
-  (* works but creates let binders, and passing them through an ltac that does cbv zeta
-     runs into the same error *)
-
-  epose ((fun (a: nat) (b: nat) (c: nat) => fun f => f (a * b * c)) _ _ _).
-  (* like with let binders, but would need to do cbv beta *)
-
-  epose (match  _: nat, _: nat, _: nat with
-         | a, b, c => a * b * c
-         end).
-  (* works, but names are too far apart from their types *)
-
-  epose (??a: nat in (a * a)).
-  epose (??a: nat in ??b: nat in (a * b)).
-  epose (??a: Z in ??b: Z in ??c: Z in (a * b * c)).
-  (* best workaround so far *)
-Abort.
-
-(* Tests:
-
-Goal False.
-  has_type 4%nat nat.
-  let T := open_constr:(_: Type) in has_type 3 T; idtac T.
-  Fail has_type 4%nat unit.
-  has_type nat Set.
-  has_type nat Type.
-  has_type (fun (x: Set) => (x * x)%type) (Set -> Set).
-  has_type (fun (x: Type) => (x * x)%type) (Set -> Set).
-  has_type (fun (x: Type) => (x * x)%type) (Set -> Type).
-  Fail has_type (fun (x: Set) => (x * x)%type) (Type -> Type).
-  Fail has_type (fun (x: Set) => (x * x)%type) (Type -> Set).
-Abort.
-
-Fail Check (fun a b => a * b).
-Fail Check (fun a (b: Z) => a * b).
-Fail Check (fun (a: nat) b => a * b).
-Check (fun (a b: nat) => a * b).
-Fail Check (fun (a: nat) (b: Z) => a * b).
-Fail Check (tt * 2).
-Fail Check (tt * tt).
-Check (nat * Z)%type.
-Check (nat * Z).
-Check (nat * Set).
-Check (nat * Type).
-
-Section WithParameters.
-  Context {word: word.word 32} {mem: map.map word Byte.byte}.
-  Context {word_ok: word.ok word} {mem_ok: map.ok mem}.
-
-  Check (fun (P Q: mem -> Prop) => P * Q).
-
-  Local Coercion Z.of_nat : nat >-> Z.
-  Local Coercion word.unsigned : word.rep >-> Z.
-
-(*  Local Set Printing Coercions.*)
-
-  Check (fun (x: word) => x: Z).
-  Check (fun (x: nat) => x: Z).
-
-  (*
-  New coercion path [word_to_nat; Z.of_nat] : word.rep >-> Z is ambiguous with existing
-  [word.unsigned] : word.rep >-> Z. [ambiguous-paths,typechecker]
-  Coercion word_to_nat(w: word): nat := Z.to_nat (word.unsigned w).
-  *)
-
-  Check (fun (a: nat) (b: Z) => a * b).
-  Check (fun (a: Z) (b: nat) => a * b).
-  Check (fun (a: Z) (b: nat) (c: Z) => a * b * c).
-  Check (fun (a b c: Z) => a * b * c).
-  Check (fun (a: nat) (b: nat) (c: Z) => a * b * c).
-
-  Fail Check (fun (x: word) (y: mem -> Prop) => x * y).
-
-  Check (fun (P Q R: mem -> Prop) m => (P * Q * R) m).
-End WithParameters.
-*)
+  Goal forall (a1 a2 ofs sz v1 v2: word) (R: mem -> Prop) (m: mem), (R * R) m. Abort.
+  Goal forall (a1 a2 ofs sz v1 v2: word) (R: mem -> Prop) (m: mem), (a1 |-> v1) m. Abort.
+  Goal forall (a1 a2 ofs sz v1 v2: word) (R: mem -> Prop) (m: mem),
+      (R * a1 |-> v1) m.
+  Abort.
+  Goal forall (a1 a2 ofs sz v1 v2: word) (R: mem -> Prop) (m: mem),
+      ((a1 |-> v1) * R) m.
+  Abort.
+  Goal forall (a1 a2 ofs sz v1 v2: word) (R: mem -> Prop) (m: mem),
+      (a1 |-> v1 * a2 |-> v2 * R) m.
+    intros.
+  Abort.
+  Goal forall (a1 a2 ofs sz v1 v2: word) (R: mem -> Prop) (m: mem),
+      ((a1 + ofs * sz) |-> v1 * a2 |-> v2 * R) m.
+    intros.
+  Abort.
+End TestNotations.
